src/SeqRec.lean
@@ -2,7 +2,7 @@ import Utility tactic
 
 --Logic Unit 2
 def LUT2 (Q1 Q0 X : bool) : bool :=
-  OR [AND [Q1, Q0, X], AND [Q1, NOT Q0 , X], AND[NOT Q1, Q0, X], AND[NOT Q1, NOT Q0, X]]
+  OR [AND [Q1, Q0, X], AND [Q1, NOT Q0, X], AND[NOT Q1, Q0, X], AND[NOT Q1, NOT Q0, X]]
 
 def LUT2_spec (Q1 Q0 X OUT : bool) : Prop :=
   if (¬Q1 ∧ ¬Q0 ∧ X) ∨ (¬Q1 ∧ Q0 ∧ X) ∨ (Q1 ∧ ¬Q0 ∧ X) ∨ (Q1 ∧ Q0 ∧ X) then OUT = tt
@@ -23,7 +23,7 @@ theorem LUT2_correct : ∀ (Q1 Q0 X : bool),
 
 --Logic Unit 3
 def LUT3 (Q1 Q0 X : bool) : bool :=
-  OR [AND [NOT Q1, Q0, NOT X], AND [Q1, NOT Q0 , X], AND [Q1, Q0, X]]
+  OR [AND [NOT Q1, Q0, NOT X], AND [Q1, NOT Q0, X], AND [Q1, Q0, X]]
 
 
 def LUT3_spec (Q1 Q0 X OUT : bool) : Prop :=
@@ -31,7 +31,7 @@ def LUT3_spec (Q1 Q0 X OUT : bool) : Prop :=
   else OUT = ff
 
 theorem LUT3_correct : ∀ (Q1 Q0 X : bool),
-  ∀ (OUT : bool), LUT3_spec Q1 Q0 X OUT ↔ LUT3 Q1 Q0 X  = OUT :=
+  ∀ (OUT : bool), LUT3_spec Q1 Q0 X OUT ↔ LUT3 Q1 Q0 X = OUT :=
   begin
     intros,
     unfold LUT3_spec LUT3,
@@ -66,94 +66,77 @@ theorem LUT0_correct : ∀ (Q1 Q0 : bool), ∀ (OUT : bool),
 --Complete circuit
 def SeqRecAux {n : ℕ} (X : signal) : Π (i : ℕ), i ≤ n → bool → bool → bool → ℕ → bool
   |(nat.zero) h Q1 Q0 O k :=
-    if k ≤ 3 then
-      let Q1_next := LUT3 Q1 Q0 (X 0),
-          Q0_next := LUT2 Q1 Q0 (X 0),
-          O_next := LUT0 Q1_next Q0_next in
-      if O = tt then tt
-      else ff
+    if O = tt then tt
     else ff
   |(nat.succ t) h Q1 Q0 O k :=
-    if k ≤ 3 then
+    if O = tt then tt
+    else if k < 3 then
       let Q1_next := LUT3 Q1 Q0 (X t),
           Q0_next := LUT2 Q1 Q0 (X t),
           O_next := LUT0 Q1_next Q0_next in
-      if O = tt then tt
-      else if k = 3 then ff
-      else SeqRecAux (t) (le_of_lt h) Q1_next Q0_next (O_next) (k+1)
+      SeqRecAux (t) (le_of_lt h) Q1_next Q0_next (O_next) (k+1)
     else ff
 
 def SeqRec (X : signal) : signal :=
   λ n, SeqRecAux X (n) (le_refl _) ff ff ff 0
 
-def SeqRec_spec (X OUT : ℕ → bool) : Prop :=
+def SeqRec_spec (X OUT : signal) : Prop :=
   ∀ t : ℕ, 
     (X t = tt → X (t+1) = ff → X (t+2) = tt → OUT (t+3) = tt) ∧ 
+    (X t = tt → X (t+1) = tt → X (t+2) = tt → OUT (t+3) = ff) ∧ 
+    (X t = tt → X (t+1) = tt → X (t+2) = ff → OUT (t+3) = ff) ∧ 
+    (X t = tt → X (t+1) = ff → X (t+2) = ff → OUT (t+3) = ff) ∧ 
     (X t = ff → OUT (t+3) = ff)
 
-def SeqReq_correct : ∀ (X : ℕ → bool),
+
+theorem SeqReq_correct : ∀ (X : signal),
   SeqRec_spec X (SeqRec X) :=
   begin
     intros X,
     unfold SeqRec_spec,
     intros t,
-    split,
-    {
+    repeat{
+      split,
       intros h₁ h₂ h₃,
       unfold SeqRec,
       repeat {
         unfold SeqRecAux,
         simp,
       },
-      unfold LUT0 LUT3 LUT2 OR AND,
-      simp,
-      unfold NOT,
-      simp,
+      simp [LUT0, LUT2, LUT3, AND, OR, NOT],
       rw h₃,
       rw h₂,
-      simp,
-      unfold NOT,
-      simp,
       rw h₁,
+      simp [NOT],
       ring_nf,
       simp,
-      cases t,
+      cases t;
       {
         unfold SeqRecAux,
-        simp,
+        refl,
+        try {unfold NOT},
       },
-      {
-        unfold SeqRecAux,
-        simp,
-      }
     },
+    intro h₁,
+    unfold SeqRec,
+    repeat {
+      unfold SeqRecAux,
+      simp,
+    },
+    simp [LUT0, LUT2, LUT3, AND, OR, NOT],
+    cases X (t+1); cases X(t+2);
     {
-      intro h₁,
-      unfold SeqRec,
-      repeat {
-        unfold SeqRecAux,
-        simp,
-      },
-      simp [LUT0, LUT2, LUT3, AND, OR, NOT],
-      cases X (t+1); cases X(t+2);
+      simp [NOT],
+      ring_nf,
+      simp,
+      cases t;
       {
-        simp [NOT],
-        ring_nf,
-        simp,
-        cases t,
-        {
-          unfold SeqRecAux,
-          finish,
-        },
-        {
-          unfold SeqRecAux,
-          finish,
-        }
-      }
-    },
+        unfold SeqRecAux,
+        finish,
+      },
+    }, 
   end
 
 --Example
 def X : signal := λx,x=0 ∨ x = 2 ∨ x = 4 ∨ x = 6 ∨ x=8 ∨ x=15 ∨ x = 17 
-#eval (SeqRec X) 
-
+#eval (SeqRec X) 18
